code/ecdsap256sha2/Hacl.Impl.ECDSA.fsti
@@ -38,6 +38,7 @@ open Hacl.Impl.ECDSA.P256SHA256.Verification.Agile
 open Hacl.Impl.ECDSA.P256SHA256.Verification.Hashless
 
 open Spec.P256.MontgomeryMultiplication
+open Hacl.Impl.ECDSA.Reduction
 
 
 val ecdsa_sign_p256_sha2: result: lbuffer uint8 (size 64) -> mLen: size_t -> m: lbuffer uint8 mLen ->
@@ -265,3 +266,11 @@ val compressionCompressedForm: b: lbuffer uint8 (size 64) -> result: compressedF
       )  
   )
 
+
+val reduction_8_32: x: lbuffer uint8 (size 32) -> result: lbuffer uint8 (size 32) -> 
+  Stack unit 
+    (requires fun h -> live h x /\ live h result /\ eq_or_disjoint x result)
+    (ensures fun h0 _ h1 -> modifies (loc result) h0 h1 /\ 
+      nat_from_bytes_be (as_seq h1 result) == nat_from_bytes_be (as_seq h0 x) % prime_p256_order /\
+      nat_from_bytes_be (as_seq h1 result) < prime_p256_order
+    )
